concurrent hash example

theories/coneris/examples/hash.v
@@ -1,12 +1,12 @@
-From clutch.coneris Require Export coneris lib.map.
-From iris.algebra Require Import excl_auth numbers.
 From stdpp Require Export fin_maps.
+From iris.algebra Require Import excl_auth numbers gset_bij.
+From clutch.coneris Require Export coneris lib.map.
 Import Hierarchy.
 Set Default Proof Using "Type*".
 
 Section simple_bit_hash.
 
-  Context `{!conerisGS Σ}.
+  Context `{!conerisGS Σ, HinG: inG Σ (gset_bijR nat nat)}.
 
   Variable val_size : nat.
 
@@ -49,6 +49,81 @@ Section simple_bit_hash.
     is_Some (m !! k2) ->
     m !!! k1 = m !!! k2 ->
     k1 = k2.
+  
+  Definition hash_view_auth m γ := (own γ (gset_bij_auth (DfracOwn 1) (map_to_set pair m)))%I.
+  Definition hash_view_frag k v γ := (own γ (gset_bij_elem k v)).
+
+  Lemma hash_view_auth_coll_free m γ2:
+    hash_view_auth m γ2 -∗ ⌜coll_free m⌝.
+  Proof.
+    rewrite /hash_view_auth.
+    iIntros "H".
+    iDestruct (own_valid with "[$]") as "%H".
+    rewrite gset_bij_auth_valid in H.
+    iPureIntro.
+    intros k1 k2 H1 H2 H3.
+    destruct H1 as [v1 K1].
+    destruct H2 as [v2 H2].
+    assert (v1 = v2) as ->; first by erewrite !lookup_total_correct in H3.
+    unshelve epose proof (H k1 v2 _) as [_ H']; first by rewrite elem_of_map_to_set_pair.
+    unshelve epose proof (H' k2 _) as ->; last done.
+    by rewrite elem_of_map_to_set_pair.
+  Qed.
+
+  Lemma hash_view_auth_duplicate_frag m n b γ2:
+    m!!n=Some b -> hash_view_auth m γ2 ==∗ hash_view_auth m γ2 ∗ hash_view_frag n b γ2.
+  Proof.
+    iIntros (Hsome) "Hauth".
+    rewrite /hash_view_auth/hash_view_frag.
+    rewrite -own_op.
+    iApply own_update; last done.
+    rewrite -core_id_extract; first done.
+    apply bij_view_included.
+    rewrite elem_of_map_to_set.
+    naive_solver.
+  Qed.
+  
+  Lemma hash_view_auth_frag_agree m γ2 k v:
+    hash_view_auth m γ2  ∗ hash_view_frag k v γ2 -∗
+    ⌜m!!k=Some v⌝.
+  Proof.
+    rewrite /hash_view_auth/hash_view_frag.
+    rewrite -own_op.
+    iIntros "H".
+    iDestruct (own_valid with "[$]") as "%H".
+    rewrite bij_both_valid in H.
+    destruct H as [? H].
+    rewrite elem_of_map_to_set in H.
+    iPureIntro.
+    destruct H as (?&?&?&?).
+    by simplify_eq.
+  Qed.
+
+  Lemma hash_view_auth_insert m n x γ:
+    m!!n=None ->
+    Forall (λ m : nat, x ≠ m) (map (λ p : nat * nat, p.2) (map_to_list m)) ->
+    hash_view_auth m γ ==∗
+    hash_view_auth (<[n:=x]> m) γ ∗ hash_view_frag n x γ.
+  Proof.
+    iIntros (H1 H2) "H".
+    rewrite /hash_view_auth/hash_view_frag.
+    rewrite -own_op.
+    iApply own_update; last done.
+    rewrite -core_id_extract; last first.
+    { apply bij_view_included. rewrite elem_of_map_to_set.
+      eexists _, _; split; last done.
+      apply lookup_insert.
+    }
+    etrans; first apply gset_bij_auth_extend; last by rewrite map_to_set_insert_L.
+    - intros b. rewrite elem_of_map_to_set; intros (?&?&?&?).
+      simplify_eq.
+    - intros a. rewrite elem_of_map_to_set; intros (?&?&?&?).
+      simplify_eq.
+      rewrite Forall_map in H2.
+      rewrite Forall_forall in H2.
+      unfold not in H2.
+      eapply H2; [by erewrite elem_of_map_to_list|done].
+  Qed.
 
   Definition hashfun f m : iProp Σ :=
     ∃ (hm : loc), ⌜ f = compute_hash_specialized #hm ⌝ ∗
@@ -56,11 +131,11 @@ Section simple_bit_hash.
                   ⌜map_Forall (λ ind i, (0<= i <=val_size)%nat) m⌝
   .
 
-  Definition coll_free_hashfun f m: iProp Σ :=
-    hashfun f m ∗ ⌜coll_free m⌝.
+  Definition coll_free_hashfun f m γ: iProp Σ :=
+    hashfun f m ∗ hash_view_auth m γ.
 
-  Lemma coll_free_hashfun_implies_hashfun f m:
-    coll_free_hashfun f m -∗ hashfun f m.
+  Lemma coll_free_hashfun_implies_hashfun f m γ:
+    coll_free_hashfun f m γ -∗ hashfun f m.
   Proof.
     by iIntros "[??]".
   Qed.
@@ -69,14 +144,15 @@ Section simple_bit_hash.
     Timeless (hashfun f m).
   Proof. apply _. Qed.
 
-  #[global] Instance timeless_hashfun_amortized f m:
-    Timeless (coll_free_hashfun f m).
+  #[global] Instance timeless_hashfun_amortized f m γ:
+    Timeless (coll_free_hashfun f m γ).
   Proof. apply _. Qed.
 
-  Lemma coll_free_hashfun_implies_coll_free f m:
-    coll_free_hashfun f m -∗ ⌜coll_free m⌝.
+  Lemma coll_free_hashfun_implies_coll_free f m γ:
+    coll_free_hashfun f m γ-∗ ⌜coll_free m⌝.
   Proof.
-    by iIntros "[??]".
+    iIntros "[??]".
+    by iApply hash_view_auth_coll_free.
   Qed.
 
   Lemma hashfun_implies_bounded_range f m idx x:
@@ -87,17 +163,17 @@ Section simple_bit_hash.
     by eapply map_Forall_lookup_1 in K.
   Qed.
 
-  Lemma coll_free_hashfun_implies_bounded_range f m idx x:
-    coll_free_hashfun f m -∗ ⌜m!!idx = Some x⌝ -∗ ⌜(0<=x<=val_size)%nat⌝.
+  Lemma coll_free_hashfun_implies_bounded_range f m idx x γ:
+    coll_free_hashfun f m γ -∗ ⌜m!!idx = Some x⌝ -∗ ⌜(0<=x<=val_size)%nat⌝.
   Proof.
-    iIntros "(H&%) %".
+    iIntros "(H&?) %".
     by iApply (hashfun_implies_bounded_range with "[$]").
   Qed.
 
   Lemma wp_init_hash E :
     {{{ True }}}
       init_hash #() @ E
-    {{{ f, RET f; |={E}=> coll_free_hashfun f ∅ }}}.
+    {{{ f, RET f; ∃ γ, |={E}=> coll_free_hashfun f ∅ γ}}}.
   Proof.
     rewrite /init_hash.
     iIntros (Φ) "_ HΦ".
@@ -105,10 +181,12 @@ Section simple_bit_hash.
     wp_apply (wp_init_map with "[//]").
     iIntros (?) "Hm". wp_pures.
     rewrite /compute_hash. wp_pures.
-    iApply "HΦ". repeat iModIntro. rewrite /coll_free_hashfun. iSplit.
-    - iExists _. rewrite fmap_empty. iFrame. eauto.
-    - iPureIntro. rewrite /coll_free. intros ???H?. destruct H.
-      by apply lookup_empty_Some in H.
+    iAssert (|==> (∃ γ2, hash_view_auth ∅ γ2))%I as ">(%γ2 & Hview)".
+    { rewrite /hash_view_auth.
+      iApply own_alloc.
+      by rewrite gset_bij_auth_valid.
+    }
+    iApply "HΦ". repeat iModIntro. rewrite /coll_free_hashfun. by iFrame.
   Qed.
 
   Lemma coll_free_insert (m : gmap nat nat) (n : nat) (z : nat) :
@@ -169,32 +247,45 @@ Section simple_bit_hash.
     iExists _. eauto.
   Qed.
 
-  Lemma wp_coll_free_hashfun_prev E f m (n : nat) (b : nat) :
+  
+  Lemma wp_coll_free_hashfun_prev E f m γ (n : nat) (b : nat) :
     m !! n = Some b →
-    {{{ coll_free_hashfun f m }}}
+    {{{ coll_free_hashfun f m γ }}}
       f #n @ E
-    {{{ RET #b; coll_free_hashfun f m }}}.
+    {{{ RET #b; coll_free_hashfun f m γ ∗ hash_view_frag n b γ }}}.
   Proof.
-    iIntros (Hlookup Φ) "(Hhash & %Hcoll_free) HΦ".
+    iIntros (Hlookup Φ) "(Hhash & Hauth) HΦ".
     iDestruct "Hhash" as (hm ->) "[H Hbound]".
     rewrite /compute_hash_specialized.
     wp_pures.
     wp_apply (wp_get with "[$]").
     iIntros (vret) "(Hhash&->)".
-    rewrite lookup_fmap Hlookup /=. wp_pures. iModIntro. iApply "HΦ".
-    iSplitL; last done.
-    iExists _. eauto.
+    rewrite lookup_fmap Hlookup /=. wp_pures.
+    iMod (hash_view_auth_duplicate_frag with "[$]") as "[??]"; first done.
+    iModIntro. iApply "HΦ". by iFrame.
   Qed.
 
+  Lemma wp_coll_free_hashfun_frag_prev E f m γ (n : nat) (b : nat) :
+    {{{ coll_free_hashfun f m γ ∗ hash_view_frag n b γ}}}
+      f #n @ E
+    {{{ RET #b; coll_free_hashfun f m γ }}}.
+  Proof.
+    iIntros (Φ) "[[Hhash ?] #Hfrag] HΦ".
+    iDestruct (hash_view_auth_frag_agree with "[$]") as "%".
+    iApply (wp_coll_free_hashfun_prev with "[$]"); first done.
+    iIntros "!> [??]".
+    by iApply "HΦ".
+  Qed.
+  
 
-  Lemma wp_insert_no_coll E f m (n : nat) :
+  Lemma wp_insert_no_coll E f m (n : nat) γ:
     m !! n = None →
-    {{{ coll_free_hashfun f m ∗ ↯ (nnreal_div (nnreal_nat (length (map_to_list m))) (nnreal_nat(val_size+1)))
+    {{{ coll_free_hashfun f m γ ∗ ↯ (nnreal_div (nnreal_nat (length (map_to_list m))) (nnreal_nat(val_size+1)))
     }}}
       f #n @ E
-    {{{ (v : nat), RET #v; coll_free_hashfun f (<[ n := v ]>m) }}}.
+    {{{ (v : nat), RET #v; coll_free_hashfun f (<[ n := v ]>m) γ ∗ hash_view_frag n v γ }}}.
   Proof.
-    iIntros (Hlookup Φ) "([Hhash %Hcoll_free] & Herr) HΦ".
+    iIntros (Hlookup Φ) "([Hhash Hauth] & Herr) HΦ".
     iDestruct "Hhash" as (hm ->) "[H %Hbound]".
     rewrite /compute_hash_specialized.
     wp_pures.
@@ -211,32 +302,36 @@ Section simple_bit_hash.
     wp_apply (wp_set with "Hhash").
     iIntros "Hlist".
     wp_pures.
+    iMod (hash_view_auth_insert with "[$]") as "[??]"; [done..|].
     iModIntro.
     iApply "HΦ".
-    iSplit.
-    - rewrite /hashfun.
-      iExists _.
-      iSplit; first auto.
-      iSplitL.
-      + rewrite fmap_insert //.
-      + iPureIntro.
-        apply map_Forall_insert_2; last done.
-        split.
-        * lia.
-        * pose proof (fin_to_nat_lt x).
-          lia.
+    iFrame.
+    rewrite /hashfun.
+    iExists _.
+    iSplit; first auto.
+    iSplitL.
+    - rewrite fmap_insert //.
     - iPureIntro.
-      apply coll_free_insert; auto.
-      apply (Forall_map (λ p : nat * nat, p.2)) in HForall; auto.
+      apply map_Forall_insert_2; last done.
+      split.
+      + lia.
+      + pose proof (fin_to_nat_lt x).
+        lia.
   Qed.
-
 
 End simple_bit_hash.
 
 
 
 Section amortized_hash.
-  Context `{!conerisGS Σ, HinG: inG Σ (authR natR)}.
+
+  Class amortized_hashG Σ :=
+    {
+        amortized_hash_credit :: inG Σ (authR natR) ;
+        amortized_hash_gset_bij :: inG Σ (gset_bijR nat nat)
+      }.
+       
+  Context `{!conerisGS Σ, Hah: amortized_hashG Σ}.
   Variable val_size:nat.
   Variable max_hash_size : nat.
   Hypothesis max_hash_size_pos: (0<max_hash_size)%nat.
@@ -251,27 +346,34 @@ Section amortized_hash.
     replace 1 with (INR 1); last simpl; [by apply le_INR|done].
   Qed.
 
+  
   Definition hashfun_amortized f m γ: iProp Σ :=
     ∃ (k : nat) (ε : nonnegreal),
       hashfun val_size f m ∗
       ⌜k = size m⌝ ∗
       ⌜ (ε.(nonneg) = (((max_hash_size-1) * k)/2 - sum_n_m (λ x, INR x) 0%nat (k-1)) / (val_size + 1))%R⌝ ∗
       ↯ ε ∗
+      (** token *)
       own γ (● max_hash_size) ∗
-      own γ (◯ k)
+      own γ (◯ k) 
   .
 
-  Definition coll_free_hashfun_amortized f m γ: iProp Σ :=
-    hashfun_amortized f m γ ∗ ⌜coll_free m⌝.
+  
+  Definition coll_free_hashfun_amortized f m γ1 γ2: iProp Σ :=
+    hashfun_amortized f m γ1 ∗
+      (** gset_bij *)
+      hash_view_auth m γ2.
 
   #[global] Instance timeless_coll_free_hashfun_amortized f m γ:
     Timeless (hashfun_amortized f m γ).
   Proof. apply _. Qed.
 
-  Lemma coll_free_hashfun_amortized_implies_coll_free f m γ:
-    coll_free_hashfun_amortized f m γ -∗ ⌜coll_free m⌝.
+
+  Lemma coll_free_hashfun_amortized_implies_coll_free f m γ1 γ2:
+    coll_free_hashfun_amortized f m γ1 γ2 -∗ ⌜coll_free m⌝.
   Proof.
-    by iIntros "[??]".
+    iIntros "[??]".
+    by iApply hash_view_auth_coll_free. 
   Qed.
 
   Lemma hashfun_amortized_implies_bounded_range f m γ idx x:
@@ -281,32 +383,32 @@ Section amortized_hash.
     iApply (hashfun_implies_bounded_range with "[H]"); [by iDestruct "H" as "(%&%&H&H')"|done].
   Qed.
 
-  Lemma coll_free_hashfun_amortized_implies_bounded_range f m γ idx x:
-    coll_free_hashfun_amortized f m γ -∗ ⌜m!!idx = Some x⌝ -∗ ⌜(0<=x<=val_size)%nat⌝.
+  Lemma coll_free_hashfun_amortized_implies_bounded_range f m γ1 γ2 idx x:
+    coll_free_hashfun_amortized f m γ1 γ2 -∗ ⌜m!!idx = Some x⌝ -∗ ⌜(0<=x<=val_size)%nat⌝.
   Proof.
-    iIntros "(H&%) %".
+    iIntros "(H&?) %".
     by iApply (hashfun_amortized_implies_bounded_range with "[$]").
   Qed.
 
   Lemma wp_init_hash_amortized E :
     {{{ True }}}
       init_hash val_size #() @ E
-      {{{ f, RET f; |={E}=> ∃ γ,  coll_free_hashfun_amortized f ∅ γ ∗ own γ (◯ max_hash_size) }}}.
+      {{{ f, RET f; |={E}=> ∃ γ1 γ2,  coll_free_hashfun_amortized f ∅ γ1 γ2 ∗ own γ1 (◯ max_hash_size) }}}.
   Proof.
     iIntros (Φ) "_ HΦ".
     wp_apply wp_init_hash; first done.
-    iIntros (f) "H".
+    iIntros (f) "(%γ2&H)".
     iApply "HΦ".
     iMod ec_zero.
     iMod "H".
-    iMod (own_alloc (● max_hash_size ⋅ ◯ (0+max_hash_size)%nat)) as (γ) "[H● [? H◯]]"; first (simpl; by apply auth_both_valid_2).
+    iMod (own_alloc (● max_hash_size ⋅ ◯ (0+max_hash_size)%nat)) as (γ1) "[H● [? H◯]]"; first (simpl; by apply auth_both_valid_2).
     iModIntro.
-    iExists _.
+    iExists _, _.
     iSplitR "H◯"; last done.
-    iSplit; last by iApply coll_free_hashfun_implies_coll_free.
     iDestruct "H" as "[??]".
-    iExists 0%nat, nnreal_zero.
+    (* iExists 0%nat, nnreal_zero. *)
     iFrame.
+    iExists nnreal_zero.
     repeat (iSplit; [done|]). iFrame.
     iPureIntro.
     simpl.
@@ -324,7 +426,7 @@ Section amortized_hash.
     m !! n = Some b →
     {{{ hashfun_amortized f m γ }}}
       f #n @ E
-      {{{ RET #b; hashfun_amortized f m γ }}}.
+      {{{ RET #b; hashfun_amortized f m γ}}}.
   Proof.
     iIntros (Hlookup Φ) "(%&%&Hhash&->&%&Herr) HΦ".
     wp_apply (wp_hashfun_prev with "[$Hhash]"); [done|].
@@ -332,18 +434,31 @@ Section amortized_hash.
     iExists _, _. iFrame. naive_solver.
   Qed.
 
-  Lemma wp_coll_free_hashfun_prev_amortized E f m γ (n : nat) (b : nat) :
+  Lemma wp_coll_free_hashfun_prev_amortized E f m γ1 γ2 (n : nat) (b : nat) :
     m !! n = Some b →
-    {{{ coll_free_hashfun_amortized f m γ }}}
+    {{{ coll_free_hashfun_amortized f m γ1 γ2 }}}
       f #n @ E
-      {{{ RET #b; coll_free_hashfun_amortized f m γ }}}.
+      {{{ RET #b; coll_free_hashfun_amortized f m γ1 γ2 ∗ hash_view_frag n b γ2 }}}.
   Proof.
-    iIntros (Hlookup Φ) "[H %Hcoll_free] HΦ".
+    iIntros (Hlookup Φ) "(H & Hauth) HΦ".
+    iMod (hash_view_auth_duplicate_frag with "[$]") as "[??]"; first done.
     wp_apply (wp_hashfun_prev_amortized with "[$]"); [done|].
     iIntros "H". iApply "HΦ".
-    by iSplitL.
+    by iFrame. 
   Qed.
 
+  
+  Lemma wp_coll_free_hashfun_prev_frag_amortized E f m γ1 γ2 (n : nat) (b : nat) :
+    {{{ coll_free_hashfun_amortized f m γ1 γ2 ∗ hash_view_frag n b γ2 }}}
+      f #n @ E
+      {{{ RET #b; coll_free_hashfun_amortized f m γ1 γ2 }}}.
+  Proof.
+    iIntros (Φ) "([??] & #H') HΦ".
+    iDestruct (hash_view_auth_frag_agree with "[$]") as "%".
+    iApply (wp_coll_free_hashfun_prev_amortized with "[$]"); first done.
+    iIntros "!> [??]".
+    by iApply "HΦ".
+  Qed.
 
   Lemma amortized_inequality (k : nat):
     (k <= max_hash_size)%nat ->
@@ -399,14 +514,14 @@ Section amortized_hash.
     rewrite nat_op in H'. lia.
   Qed.
 
-  Lemma wp_insert_new_amortized E f m γ (n : nat) :
+  Lemma wp_insert_new_amortized E f m γ1 γ2  (n : nat) :
     m !! n = None →
     (size m < max_hash_size)%nat ->
-    {{{ coll_free_hashfun_amortized f m γ∗ ↯ amortized_error ∗ own γ (◯ 1%nat)}}}
+    {{{ coll_free_hashfun_amortized f m γ1 γ2 ∗ ↯ amortized_error ∗ own γ1 (◯ 1%nat)}}}
       f #n @ E
-      {{{ (v : nat), RET #v; coll_free_hashfun_amortized f (<[ n := v ]>m) γ }}}.
+      {{{ (v : nat), RET #v; coll_free_hashfun_amortized f (<[ n := v ]>m) γ1 γ2 ∗ hash_view_frag n v γ2}}}.
   Proof.
-    iIntros (Hlookup Hineq Φ) "([Hhash %Hcoll_free] & Herr & Htoken) HΦ".
+    iIntros (Hlookup Hineq Φ) "([Hhash Hview] & Herr & Htoken) HΦ".
     iDestruct (hashfun_amortized_token_ineq with "[$Hhash][$]") as "%".
     iDestruct "Hhash" as (k ε) "(H&->&%H0&Herr'& Hauth &Hfrag)".
     set (ε' := (((max_hash_size-1) * size (<[n:=0%nat]> m) / 2 -
@@ -464,13 +579,11 @@ Section amortized_hash.
         rewrite -{2}(Rmult_1_r (h-1)).
         rewrite -Rmult_plus_distr_l.
         f_equal.
-    - wp_apply (wp_insert_no_coll with "[H Hε]"); [done|..].
-      + rewrite map_to_list_length. iFrame. done.
-      + iIntros (v) "[H %]".
+    - wp_apply (wp_insert_no_coll with "[H Hε Hview]"); [done|..].
+      + rewrite map_to_list_length. iFrame. 
+      + iIntros (v) "[[??] ?]".
         iApply "HΦ".
-        iSplitL; last done.
         iCombine "Hfrag Htoken" as "Hfrag".
-        iExists _, _.
         iFrame.
         rewrite !map_size_insert Hlookup.
         iPureIntro. split; first lia.
@@ -479,19 +592,19 @@ Section amortized_hash.
         rewrite S_INR plus_INR; simpl; lra.
   Qed.
 
-  Lemma wp_insert_amortized E f m γ (n : nat) :
-    {{{ coll_free_hashfun_amortized f m γ ∗ ↯ amortized_error ∗ own γ (◯ 1%nat)}}}
+  Lemma wp_insert_amortized E f m γ1 γ2 (n : nat) :
+    {{{ coll_free_hashfun_amortized f m γ1 γ2 ∗ ↯ amortized_error ∗ own γ1 (◯ 1%nat)}}}
       f #n @ E
-      {{{ (v : nat), RET #v; ∃ m', coll_free_hashfun_amortized f m' γ ∗ ⌜m'!!n = Some v⌝ ∗ ⌜(size m' <= S $ size(m))%nat⌝ ∗ ⌜m⊆m'⌝ }}}.
+      {{{ (v : nat), RET #v; ∃ m', coll_free_hashfun_amortized f m' γ1 γ2 ∗ ⌜m'!!n = Some v⌝ ∗ ⌜(size m' <= S $ size(m))%nat⌝ ∗ ⌜m⊆m'⌝ ∗ hash_view_frag n v γ2 }}}.
   Proof.
-    iIntros (Φ) "([Hh %Hc]& Herr & Hfrag) HΦ".
+    iIntros (Φ) "([Hh Hview]& Herr & Hfrag) HΦ".
     iDestruct (hashfun_amortized_token_ineq with "[$Hh][$]") as "%".
     destruct (m!!n) eqn:Heq.
-    - wp_apply (wp_hashfun_prev_amortized with "[$Hh]"); first done.
+    - wp_apply (wp_coll_free_hashfun_prev_amortized with "[$Hh $Hview]") as "[??]"; first done.
       iIntros. iApply "HΦ".
       iExists _; iFrame.
       repeat iSplit; try done. iPureIntro; lia.
-    - wp_apply (wp_insert_new_amortized with "[$Hh $Herr $Hfrag]"); try done.
+    - wp_apply (wp_insert_new_amortized with "[$Hh $Herr $Hfrag $Hview]"); try done.
       iIntros (?) "[??]"; iApply "HΦ".
       iExists _; iFrame. iPureIntro. repeat split.
       + rewrite lookup_insert_Some. naive_solver.
@@ -499,4 +612,8 @@ Section amortized_hash.
       + by apply insert_subseteq.
   Qed.
 
+  
+  
 End amortized_hash.
+
+  
